src/Parsers/Reflective/ParserLogicalRelations.v
@@ -1,0 +1,62 @@
+Require Import Coq.Classes.Morphisms Coq.Setoids.Setoid.
+Require Import Fiat.Parsers.Reflective.Syntax Fiat.Parsers.Reflective.Semantics.
+Require Import Fiat.Parsers.Reflective.PartialUnfold.
+Require Import Fiat.Parsers.Reflective.SyntaxEquivalence.
+Require Import Fiat.Parsers.Reflective.ParserSyntax Fiat.Parsers.Reflective.ParserSemantics.
+Require Import Fiat.Parsers.Reflective.ParserPartialUnfold.
+Require Import Fiat.Parsers.Reflective.ParserSyntaxEquivalence.
+Require Import Fiat.Parsers.Reflective.LogicalRelations.
+Require Import Fiat.Common.List.ListFacts.
+Require Import Fiat.Common.Equality.
+Require Import Fiat.Common.List.ListMorphisms.
+Require Import Fiat.Common.Wf2.
+
+Definition extract_Term {var} (E : has_parse_term var) : Term var _
+  := match E with
+     | RFix2 G_length up_to_G_length f valid_len valids nt_idx
+       => f
+     end.
+
+Theorem polypnormalize_correct
+        (is_valid_nonterminal : list nat -> nat -> bool)
+        (strlen : nat)
+        (char_at_matches : nat -> (Ascii.ascii -> bool) -> bool)
+        (split_string_for_production : nat * (nat * nat) -> nat -> nat -> list nat)
+  : forall (E : polyhas_parse_term),
+    has_parse_term_equiv nil (E interp_TypeCode) (E (normalized_of interp_TypeCode))
+    -> interp_has_parse_term
+         is_valid_nonterminal strlen char_at_matches split_string_for_production
+         (E _)
+       = interp_has_parse_term
+           is_valid_nonterminal strlen char_at_matches split_string_for_production
+           (polypnormalize E _).
+Proof.
+  intros E H.
+  unfold polypnormalize, pnormalize.
+  pose proof (fun H => @polynormalize_correct _ (fun var => extract_Term (E _)) H) as H''.
+  unfold extract_Term in *.
+  unfold polynormalize in *.
+  destruct H; simpl.
+  repeat match goal with
+         | [ H : _ /\ _ |- _ ] => destruct H
+         | [ H : ?A -> ?B, H' : ?A |- _ ] => specialize (H H')
+         end.
+  refine (Fix2_5_Proper_eq _ _ _ _ _ _ _ _ _ _);
+    unfold forall_relation, pointwise_relation;
+    repeat intro.
+  rewrite <- H''.
+  unfold step_option_rec.
+  edestruct Compare_dec.lt_dec; simpl;
+    [
+    | edestruct Sumbool.sumbool_of_bool; simpl; [ | reflexivity ] ].
+  (*
+    rewrite H''.
+    Focus 2.
+  { change (fun x => ?f x) with f.
+    simpl in *.
+
+  unfold interp_has_parse_term.
+  unfold interp_Term, polynormalize, normalize; eauto.*)
+  admit.
+  admit.
+Qed.
