src/Parsers/Reflective/ParserSoundness.v
@@ -6,6 +6,7 @@ Require Import Fiat.Parsers.Reflective.Semantics.
 Require Import Fiat.Parsers.Reflective.ParserSemantics.
 Require Import Fiat.Parsers.Reflective.PartialUnfold.
 Require Import Fiat.Parsers.Reflective.ParserPartialUnfold.
+Require Import Fiat.Parsers.Reflective.ParserLogicalRelations.
 Set Implicit Arguments.
 
 Section polypnormalize.
@@ -17,8 +18,12 @@ Section polypnormalize.
   Let interp := interp_has_parse_term is_valid_nonterminal strlen char_at_matches split_string_for_production.
 
   Lemma polypnormalize_correct (term : polyhas_parse_term)
-    : interp (polypnormalize term _) = interp (term _).
+    : ParserSyntaxEquivalence.has_parse_term_equiv
+        nil
+        (term interp_TypeCode) (term (normalized_of interp_TypeCode))
+      -> interp (term _) = interp (polypnormalize term _).
   Proof.
     subst interp.
-  Admitted.
+    apply polypnormalize_correct.
+  Qed.
 End polypnormalize.
